theories/common/Common.v
@@ -1,7 +1,9 @@
 (** Collect all Common together **)
 
-
+Add LoadPath "../../../template-coq-coq-8.5-coqOpam/theories" as Template.
 Require Export Template.Ast.
+
+Add LoadPath "../common" as Common.
 Require Export Common.exceptionMonad.
 Require Export Common.RandyPrelude.
 Require Export Common.AstCommon.
